prooftests/ExampleFromKamiTutorial_proofs.v
@@ -7,9 +7,9 @@ Require Import FunctionalExtensionality.
 
 Set Implicit Arguments.
 
-Theorem produce_consume_refinement (prefix: string):
-  TraceInclusion (Foo'mod (mkProduceConsume prefix (mkExtCall (prefix--"ext"))))
-                 (flattened_ModWf (module'mkProducerConsumer.wellformed_mkProducerConsumer prefix (mkExtCall (prefix--"ext")))).
+Theorem produce_consume_refinement:
+  TraceInclusion (Foo'mod (mkProduceConsume (mkExtCall)))
+                 (flattened_ModWf (module'mkProducerConsumer.wellformed_mkProducerConsumer (mkExtCall))).
 Proof.
   repeat autounfold with ModuleDefs.
     unfold TraceInclusion.
@@ -18,8 +18,8 @@ Proof.
   repeat split; auto; intros; unfold nthProp2; intros; try destruct (nth_error ls1 i) ; auto; repeat split; intros; try firstorder.
 Qed.
 
-Theorem consumer_refinement (prefix: string):
-  TraceInclusion (Consumer'mod (mkConsumer prefix (mkExtCall (prefix--"ext")))) (flattened_ModWf (module'mkConsumer.wellformed_mkConsumer prefix (mkExtCall (prefix--"ext")))).
+Theorem consumer_refinement:
+  TraceInclusion (Consumer'mod (mkConsumer (mkExtCall))) (flattened_ModWf (module'mkConsumer.wellformed_mkConsumer (mkExtCall))).
 Proof.
   repeat autounfold with ModuleDefs.
     unfold TraceInclusion.
@@ -28,9 +28,9 @@ Proof.
   repeat split; auto; intros; unfold nthProp2; intros; try destruct (nth_error ls1 i) ; auto; repeat split; intros; try firstorder.
 Qed.
 
-Theorem flattened_producer_consumer_refinement1 (prefix: string):
-  TraceInclusion (Producer'mod (mkProducer prefix (mkConsumer (prefix--"c0") (mkExtCall (prefix--"ext")))))
-		 (flattened_ModWf (module'mkProducer.wellformed_mkProducer prefix(mkConsumer (prefix--"c0") (mkExtCall (prefix--"ext"))))).
+Theorem flattened_producer_consumer_refinement1:
+  TraceInclusion (Producer'mod (mkProducer (mkConsumer (mkExtCall))))
+		 (flattened_ModWf (module'mkProducer.wellformed_mkProducer(mkConsumer (mkExtCall)))).
 Proof.
   repeat autounfold with ModuleDefs.
     unfold TraceInclusion.
@@ -39,22 +39,25 @@ Proof.
   repeat split; auto; intros; unfold nthProp2; intros; try destruct (nth_error ls1 i) ; auto; repeat split; intros; try firstorder.
 Qed.
 
-Theorem producer_consumer_refinement (prefix: string):
-  TraceInclusion (Producer'mod (mkProducerConsumer prefix (mkExtCall (prefix--"ext"))))
-                 (flattened_ModWf (module'mkProducerConsumer.wellformed_mkProducerConsumer prefix (mkExtCall (prefix--"ext")))).
+Theorem spec_impl_refinement:
+  TraceInclusion (Foo'mod (mkProduceConsume (mkExtCall)))
+                 (flatten_inline_remove (HideMeth (Producer'mod (mkProducerConsumer (mkExtCall))) "send")).
 Proof.
-  repeat autounfold with ModuleDefs.
-    unfold TraceInclusion.
-  intros.
-  exists o1, ls1.
-  repeat split; auto; intros; unfold nthProp2; intros; try destruct (nth_error ls1 i) ; auto; repeat split; intros; try firstorder.
-Qed.
 
-Theorem produce_consume_refinement (prefix: string):
-  TraceInclusion (Foo'mod (mkProduceConsume prefix (mkExtCall (prefix--"ext"))))
-                 (flattened_ModWf (module'mkProducerConsumer.wellformed_mkProducerConsumer prefix (mkExtCall (prefix--"ext")))).
-Proof.
   repeat autounfold with ModuleDefs.
+  unfold flatten_inline_remove, getHidden, inlineAll_All_mod, getAllRegisters,
+         getAllMethods, getAllRules, getRules, getRegisters, getMethods, app.
+  unfold inlineAll_All, inlineAll_Meths.
+  simpl.
+  unfold inlineSingle_Meths_pos, nth_error, map.
+  unfold inlineSingle_Meth.
+  unfold inlineSingle. simpl.
+  unfold inlineAll_Rules, inlineSingle_Rules_pos.
+  simpl.
+  unfold removeHides.
+  simpl.
+
+
     unfold TraceInclusion.
   intros.
   exists o1, ls1.
